terms/substitution4.v
@@ -2,6 +2,8 @@
 
   Copyright 2014 Cornell University
   Copyright 2015 Cornell University
+  Copyright 2016 Cornell University
+  Copyright 2017 Cornell University
 
   This file is part of VPrl (the Verified Nuprl project).
 
@@ -19,7 +21,10 @@
   along with VPrl.  If not, see <http://www.gnu.org/licenses/>.
 
 
-  Website: http://nuprl.org/html/verification/
+  Websites: http://nuprl.org/html/verification/
+            http://nuprl.org/html/Nuprl2Coq
+            https://github.com/vrahli/NuprlInCoq
+
   Authors: Abhishek Anand & Vincent Rahli
 
 *)
@@ -45,7 +50,7 @@ Lemma lsubst_aux_cons_sub_filter {o} :
     lsubst_aux t ((v,u) :: sub_filter sub [v])
     = lsubst_aux t ((v,u) :: sub).
 Proof.
-  nterm_ind t as [v|f|op bs ind] Case; introv; allsimpl; auto.
+  nterm_ind t as [v|op bs ind] Case; introv; allsimpl; auto.
 
   - Case "vterm".
     boolvar; auto.
