terms/terms_pk.v
@@ -1,6 +1,9 @@
 (*
 
   Copyright 2014 Cornell University
+  Copyright 2015 Cornell University
+  Copyright 2016 Cornell University
+  Copyright 2017 Cornell University
 
   This file is part of VPrl (the Verified Nuprl project).
 
@@ -15,10 +18,13 @@
   GNU General Public License for more details.
 
   You should have received a copy of the GNU General Public License
-  along with VPrl.  Ifnot, see <http://www.gnu.org/licenses/>.
+  along with VPrl.  If not, see <http://www.gnu.org/licenses/>.
 
 
-  Website: http://nuprl.org/html/verification/
+  Websites: http://nuprl.org/html/verification/
+            http://nuprl.org/html/Nuprl2Coq
+            https://github.com/vrahli/NuprlInCoq
+
   Authors: Abhishek Anand & Vincent Rahli
 
 *)
@@ -363,19 +369,14 @@ Lemma isvalue_like_implies1 {o} :
     -> {op : Opid
         & {bterms : list BTerm
         & t = oterm op bterms
-        # iscan_like_op op}}
-       [+] {f : ntseq & t = sterm f}.
+        # iscan_like_op op}}.
 Proof.
   introv isv.
   unfold isvalue_like in isv; repndors.
   - apply iscan_implies in isv; repndors; exrepnd; subst.
-    + left.
-      eexists; eexists; dands; eauto.
-      left; eexists; eauto.
-    + right.
-      eexists; eauto.
+    eexists; eexists; dands; eauto.
+    left; eexists; eauto.
   - apply isexc_implies2 in isv; exrepnd; subst.
-    left.
     eexists; eexists; dands; eauto.
     right; unfold isexc_op; auto.
 Qed.
