terms/terms_union.v
@@ -2,6 +2,8 @@
 
   Copyright 2014 Cornell University
   Copyright 2015 Cornell University
+  Copyright 2016 Cornell University
+  Copyright 2017 Cornell University
 
   This file is part of VPrl (the Verified Nuprl project).
 
@@ -19,7 +21,10 @@
   along with VPrl.  If not, see <http://www.gnu.org/licenses/>.
 
 
-  Website: http://nuprl.org/html/verification/
+  Websites: http://nuprl.org/html/verification/
+            http://nuprl.org/html/Nuprl2Coq
+            https://github.com/vrahli/NuprlInCoq
+
   Authors: Abhishek Anand & Vincent Rahli
 
 *)
@@ -399,7 +404,7 @@ Lemma wf_union {o} :
 Proof.
   introv; split; intro w; repnd.
   rw @wf_term_eq in w.
-  inversion w as [| | op l bwf e ]; subst.
+  inversion w as [| op l bwf e ]; subst.
   generalize (bwf (nobnd a)) (bwf (nobnd b));
     clear bwf; intros bwf1 bwf2.
   autodimp bwf1 hyp; autodimp bwf2 hyp; try (complete (simpl; sp)).
@@ -427,7 +432,7 @@ Lemma wf_decide {p} :
 Proof.
   introv; split; intro w; repnd.
   rw @wf_term_eq in w.
-  inversion w as [| | o l bwf e ]; subst.
+  inversion w as [| o l bwf e ]; subst.
   generalize (bwf (nobnd a)) (bwf (bterm [v1] b1)) (bwf (bterm [v2] b2));
     clear bwf; intros bwf1 bwf2 bwf3.
   autodimp bwf1 hyp; autodimp bwf2 hyp; autodimp bwf3 hyp; try (complete (simpl; sp)).
